src/computational_monads/simulation_semantics/constructions/logging/query_cache/add_fresh_queries.lean
@@ -1,0 +1,81 @@
+/-
+Copyright (c) 2023 Devon Tuma. All rights reserved.
+Released under Apache 2.0 license as described in the file LICENSE.
+Authors: Devon Tuma
+-/
+import computational_monads.simulation_semantics.constructions.logging.query_cache.order
+
+/-!
+# Merging Fresh Values Into a Cache
+
+This file defines a function `cache.add_fresh_queries cache'` that adds values from `cache'` to
+`cache`, assuming the value is fresh, leaving other values unchanged.
+
+If the two `query_cache`s are disjoint this acts like a sup operation, but in general doesn't
+satisfy the criteria for being a `semilattice`.
+-/
+
+
+namespace query_cache
+
+open oracle_spec oracle_comp
+
+variables {α β γ : Type} {spec spec' : oracle_spec}
+
+/-- Add queries in `s'` to `s`, for any query that is fresh to `s`.
+If the query isn't fresh preserve the value cached in `s'`.
+This behaves like a `⊔` operation if the caches have disjoint `cached_inputs` sets,
+but doesn't in general, so we choose not to implement a `has_sup` typeclass instance. -/
+def add_fresh_queries (cache cache' : query_cache spec) : query_cache spec :=
+{ cache_fn := λ i t, if cache.is_cached i t then cache.lookup i t else cache'.lookup i t,
+  cached_inputs := cache.cached_inputs ∪ cache'.cached_inputs,
+  mem_cached_inputs := λ x, by split_ifs with hx; simp [hx, mem_cached_inputs_iff_is_cached] }
+
+variables (cache cache' : query_cache spec)
+
+@[simp] lemma cached_inputs_add_fresh_queries : (cache.add_fresh_queries cache').cached_inputs =
+  cache.cached_inputs ∪ cache'.cached_inputs := rfl
+
+@[simp] lemma lookup_add_fresh_queries (i t) : (cache.add_fresh_queries cache').lookup i t =
+  if cache.is_cached i t then cache.lookup i t else cache'.lookup i t := rfl
+
+lemma lookup_add_fresh_queries_of_is_cached {i t} (h : cache.is_cached i t) :
+  (cache.add_fresh_queries cache').lookup i t = cache.lookup i t := by simp [h]
+
+@[simp] lemma lookup_add_fresh_queries_of_is_fresh {i t} (h : cache.is_fresh i t) :
+  (cache.add_fresh_queries cache').lookup i t = cache'.lookup i t :=
+by simp [not_is_cached_of_is_fresh _ h]
+
+@[simp] lemma is_fresh_add_fresh_queries_iff (i t) :
+  (cache.add_fresh_queries cache').is_fresh i t ↔ cache.is_fresh i t ∧ cache'.is_fresh i t :=
+by simp [is_fresh_iff_not_mem_cached_inputs, not_or_distrib]
+
+@[simp] lemma is_cached_add_fresh_queries_iff (i t) :
+  (cache.add_fresh_queries cache').is_cached i t ↔ cache.is_cached i t ∨ cache'.is_cached i t :=
+by simp [is_cached_iff_mem_cached_inputs]
+
+@[simp] lemma add_fresh_queries_init (cache : query_cache spec) :
+  cache.add_fresh_queries ∅ = cache :=
+by simp [query_cache.ext_iffₗ]
+
+@[simp] lemma init_add_fresh_queries (cache : query_cache spec) :
+  add_fresh_queries ∅ cache = cache :=
+by simp [query_cache.ext_iffₗ]
+
+@[simp] lemma add_fresh_queries_eq_self_iff (cache cache' : query_cache spec) :
+  cache.add_fresh_queries cache' = cache ↔ cache'.cached_inputs ⊆ cache.cached_inputs :=
+begin
+  refine ⟨λ h x hx, _, λ h, _⟩,
+  { rw [← h, cached_inputs_add_fresh_queries, finset.mem_union],
+    exact or.inr hx },
+  { refine query_cache.extₗ (λ i t, ite_eq_left_iff.2 (λ ht, _)),
+    rw [not_is_cached_iff_is_fresh] at ht,
+    exact (lookup_eq_none_of_is_fresh _ (is_fresh_of_cached_inputs_subset_of_is_fresh h ht)).trans
+      (lookup_eq_none_of_is_fresh _ ht).symm }
+end
+
+lemma add_fresh_queries_eq_self_of_le {cache cache' : query_cache spec} (h : cache' ≤ cache) :
+  cache.add_fresh_queries cache' = cache :=
+(add_fresh_queries_eq_self_iff cache cache').2 (cached_inputs_subset_cached_inputs_of_le h)
+
+end query_cache
